prove compact_digit obeys div/mod rule

src/Arithmetic/Saturated.v
@@ -105,15 +105,27 @@ Module Columns.
     Context (weight : nat->Z)
             {weight_0 : weight 0%nat = 1}
             {weight_nonzero : forall i, weight i <> 0}
+            {weight_positive : forall i, weight i > 0}
             {weight_multiples : forall i, weight (S i) mod weight i = 0}
-            (* add_get_carry takes in a number at which to split output *)
+            {weight_divides : forall i : nat, weight (S i) / weight i > 0}
+    (* add_get_carry takes in a number at which to split output *)
             {add_get_carry: Z ->Z -> Z -> (Z * Z)}
-            {add_get_carry_correct : forall s x y,
-                fst (add_get_carry s x y)  = x + y - s * snd (add_get_carry s x y)}
+            {add_get_carry_mod : forall s x y,
+                fst (add_get_carry s x y)  = (x + y) mod s}
+            {add_get_carry_div : forall s x y,
+                snd (add_get_carry s x y)  = (x + y) / s}
+            {div modulo : Z -> Z -> Z}
+            {div_correct : forall a b, div a b = a / b}
+            {modulo_correct : forall a b, modulo a b = a mod b}
     .
+    Hint Rewrite div_correct modulo_correct add_get_carry_mod add_get_carry_div : div_mod.
 
     Definition eval {n} (x : (list Z)^n) : Z :=
       B.Positional.eval weight (Tuple.map sum x).
+
+    Lemma eval_unit (x:unit) : eval (n:=0) x = 0.
+    Proof. reflexivity. Qed.
+    Hint Rewrite eval_unit : push_basesystem_eval.
 
     Definition eval_from {n} (offset:nat) (x : (list Z)^n) : Z :=
       B.Positional.eval (fun i => weight (i+offset)) (Tuple.map sum x).
@@ -138,12 +150,13 @@ Module Columns.
     Fixpoint compact_digit_cps n (digit : list Z) {T} (f:Z * Z->T) :=
       match digit with
       | nil => f (0, 0)
-      | x :: nil => f (0, x)
+      | x :: nil => f (div x (weight (S n) / weight n), modulo x (weight (S n) / weight n))
       | x :: tl =>
-        compact_digit_cps n tl (fun rec =>
-                                  dlet sum_carry := add_get_carry (weight (S n) / weight n) x (snd rec) in
-                                    dlet carry' := (fst rec + snd sum_carry)%RT in
-                                    f (carry', fst sum_carry))
+        compact_digit_cps n tl
+          (fun rec =>
+            dlet sum_carry := add_get_carry (weight (S n) / weight n) x (snd rec) in
+            dlet carry' := (fst rec + snd sum_carry)%RT in
+            f (carry', fst sum_carry))
       end.
 
     Definition compact_digit n digit := compact_digit_cps n digit id.
@@ -175,32 +188,52 @@ Module Columns.
     Lemma compact_id {n} xs {T} f : @compact_cps n xs T f = f (compact xs).
     Proof using Type. cbv [compact_cps compact]; autorewrite with uncps; reflexivity. Qed.
 
-    Lemma compact_digit_correct i (xs : list Z) :
-      snd (compact_digit i xs)  = sum xs - (weight (S i) / weight i) * (fst (compact_digit i xs)).
-    Proof using add_get_carry_correct weight_0.
+    Lemma compact_digit_mod i (xs : list Z) :
+      snd (compact_digit i xs)  = sum xs mod (weight (S i) / weight i).
+    Proof using add_get_carry_div add_get_carry_mod div_correct modulo_correct.
       induction xs; cbv [compact_digit]; simpl compact_digit_cps;
         cbv [Let_In];
         repeat match goal with
-               | _ => rewrite add_get_carry_correct
+               | _ => progress autorewrite with div_mod
+               | _ => rewrite IHxs, <-Z.add_mod_r
                | _ => progress (rewrite ?sum_cons, ?sum_nil in * )
-               | _ => progress (autorewrite with uncps push_id in * )
-               | _ => progress (autorewrite with cancel_pair in * )
+               | _ => progress (autorewrite with uncps push_id cancel_pair in * )
                | _ => progress break_match; try discriminate
-               | _ => progress ring_simplify
                | _ => reflexivity
-               | _ => nsatz
+               | _ => f_equal; ring 
                end.
+    Qed. Hint Rewrite compact_digit_mod : div_mod.
+
+    Lemma compact_digit_div i (xs : list Z) :
+      fst (compact_digit i xs)  = sum xs / (weight (S i) / weight i).
+    Proof using add_get_carry_div add_get_carry_mod div_correct modulo_correct weight_0 weight_divides.
+      induction xs; cbv [compact_digit]; simpl compact_digit_cps;
+        cbv [Let_In];
+        repeat match goal with
+               | _ => progress autorewrite with div_mod
+               | _ => rewrite IHxs
+               | _ => progress (rewrite ?sum_cons, ?sum_nil in * )
+               | _ => progress (autorewrite with uncps push_id cancel_pair in * )
+               | _ => progress break_match; try discriminate
+               | _ => reflexivity
+               | _ => f_equal; ring 
+               end.
+      assert (weight (S i) / weight i <> 0) by auto using Z.positive_is_nonzero. 
+      match goal with |- _ = (?a + ?X) / ?D =>
+                      transitivity  ((a + X mod D + D * (X / D)) / D);
+                        [| rewrite (Z.div_mod'' X D) at 3; f_equal; auto; ring]
+      end.
+      rewrite Z.div_add' by auto; nsatz.
     Qed.
 
     Definition compact_invariant n i (starter rem:Z) (inp : tuple (list Z) n) (out : tuple Z n) :=
-      B.Positional.eval_from weight i out + weight (i + n) * (rem)
-      = eval_from i inp + weight i*starter.
+      B.Positional.eval_from weight i out + weight (i + n) * rem  = eval_from i inp + weight i*starter.
 
     Lemma compact_invariant_holds n i starter rem inp out :
       compact_invariant n (S i) (fst (compact_step_cps i starter (hd inp) id)) rem (tl inp) out ->
       compact_invariant (S n) i starter rem inp (append (snd (compact_step_cps i starter (hd inp) id)) out).
     Proof using Type*.
-      cbv [compact_invariant B.Positional.eval_from]; intros.
+    cbv [compact_invariant B.Positional.eval_from]; intros.
       repeat match goal with
              | _ => rewrite B.Positional.eval_step
              | _ => rewrite eval_from_S
@@ -212,13 +245,25 @@ Module Columns.
              | _ => progress ring_simplify
              | _ => rewrite ZUtil.Z.mul_div_eq_full by apply weight_nonzero
              | _ => cbv [compact_step_cps] in *;
-                      autorewrite with uncps push_id;
-                      rewrite compact_digit_correct
+                      autorewrite with uncps push_id in *;
+                      rewrite !compact_digit_mod, !compact_digit_div in *
              | _ => progress (autorewrite with natsimplify in * )
-             end.
+             end;
       rewrite B.Positional.eval_wt_equiv with (wtb := fun i0 => weight (i0 + S i)) by (intros; f_equal; try omega).
+    {
+      rewrite Z.mod_eq by auto using Z.positive_is_nonzero.
+      rewrite sum_cons in H.
+      ring_simplify.
+      match type of H with
+        context [?y * (?a / (?y / ?x))] =>
+        replace (y * (a / (y / x))) with (x * (y / x) * (a / (y / x))) in H
+          by (rewrite Z.mul_div_eq_full by auto using Z.positive_is_nonzero;
+              rewrite weight_multiples; ring)
+      end.
       nsatz.
+    }
     Qed.
+
 
     Lemma compact_invariant_base i rem : compact_invariant 0 i rem rem tt tt.
     Proof using Type. cbv [compact_invariant]. simpl. repeat (f_equal; try omega). Qed.
@@ -366,14 +411,21 @@ Hint Rewrite
   using (assumption || omega): push_basesystem_eval.
 
 Section Freeze.
-  Context (weight : nat->Z)
-          {weight_0 : weight 0%nat = 1}
-          {weight_nonzero : forall i, weight i <> 0}
-          {weight_multiples : forall i, weight (S i) mod weight i = 0}
-          (* add_get_carry takes in a number at which to split output *)
-          {add_get_carry: Z ->Z -> Z -> (Z * Z)}
-          {add_get_carry_correct : forall s x y,
-              fst (add_get_carry s x y)  = x + y - s * snd (add_get_carry s x y)}
+    Context (weight : nat->Z)
+            {weight_0 : weight 0%nat = 1}
+            {weight_nonzero : forall i, weight i <> 0}
+            {weight_positive : forall i, weight i > 0}
+            {weight_multiples : forall i, weight (S i) mod weight i = 0}
+            {weight_divides : forall i : nat, weight (S i) / weight i > 0}
+            (* add_get_carry takes in a number at which to split output *)
+            {add_get_carry: Z ->Z -> Z -> (Z * Z)}
+            {add_get_carry_mod : forall s x y,
+                fst (add_get_carry s x y)  = (x + y) mod s}
+            {add_get_carry_div : forall s x y,
+                snd (add_get_carry s x y)  = (x + y) / s}
+            {div modulo : Z -> Z -> Z}
+            {div_correct : forall a b, div a b = a / b}
+            {modulo_correct : forall a b, modulo a b = a mod b}
   .
 
   (* adds p and q if cond is 0, else adds 0 to p*)
@@ -397,7 +449,7 @@ Section Freeze.
   Definition conditional_add_cps {n} mask cond (p q : Z^n) {T} (f:_->T) :=
     conditional_mask_cps mask cond q
     (fun qq => Columns.add_cps weight p qq
-    (fun R => Columns.compact_cps (add_get_carry:=add_get_carry) weight R f)).
+    (fun R => Columns.compact_cps (div:=div) (modulo:=modulo) (add_get_carry:=add_get_carry) weight R f)).
   Definition conditional_add {n} mask cond p q :=
     @conditional_add_cps n mask cond p q _ id.
   Lemma conditional_add_id {n} mask cond p q T f:
@@ -430,12 +482,10 @@ Section Freeze.
     B.Positional.carry_reduce_cps
       (div:=div) (modulo:=modulo) weight s c p
       (fun P => Columns.sub_cps weight P m
-      (fun Q => Columns.compact_cps (add_get_carry:=add_get_carry) weight Q
+      (fun Q => Columns.compact_cps (div:=div) (modulo:=modulo) (add_get_carry:=add_get_carry) weight Q
       (fun carry_q => conditional_add_cps mask (fst carry_q) (snd carry_q) m
       (fun carry_r => f (snd carry_r)))))
   .
-
-  SearchAbout (((_ mod _) mod _)).
 
   Definition freeze {n} mask s c m p :=
     @freeze_cps n mask s c m p _ id.
@@ -483,27 +533,27 @@ Section Freeze.
   Hint Rewrite @eval_conditional_add using (omega || assumption)
     : push_basesystem_eval.
 
-  Lemma freezeZ m s c y0 z z0 c0 a :
+  Lemma freezeZ m s c y y0 z z0 c0 a :
     m = s - c ->
     0 < c < s ->
     s <> 0 ->
-    -m <= y0 < m ->
+    0 <= y < 2*m ->
+    y0 = y - m ->
     z = y0 mod s ->
     c0 = y0 / s ->
     c0 <> 0 ->
-    z0 = z + m ->
+    z0 = z + (if (dec (c0 = 0)) then 0 else m) ->
     a = z0 mod s ->
     a mod m = y0 mod m.
   Proof.
-    clear. intros. subst.
-    rewrite Z.add_mod by assumption.
-    rewrite Z.mod_mod by assumption.
-    rewrite <-Z.add_mod by assumption.
-    assert (~ (0 <= y0 < s)) by (pose proof (Z.div_small y0 s); tauto).
-    assert (-(s-c) <= y0 < 0) by omega.
-    rewrite Z.mod_small with (b := s) by omega.
-    rewrite Z.add_mod, Z.mod_same, Z.add_0_r, Z.mod_mod by omega.
-    reflexivity.
+    clear. intros. subst. break_match.
+    { rewrite Z.add_0_r, Z.mod_mod, !Z.mod_small by omega.
+      reflexivity. }
+    { rewrite <-Z.add_mod_l, Z.sub_mod_full.
+      rewrite Z.mod_same, Z.sub_0_r, Z.mod_mod by omega.
+      rewrite Z.mod_small with (b := s)
+      by (pose proof (Z.div_small (y - (s-c)) s); omega).
+      f_equal. ring. }
   Qed.
 
   Lemma eval_freeze {n} mask s c m p
@@ -517,43 +567,23 @@ Section Freeze.
              (B.Positional.eval weight (@freeze n mask s c m p))
              (B.Positional.eval weight p).
   Proof.
-    cbv [freeze_cps freeze mod_eq]; repeat progress autounfold;
-      autorewrite with uncps push_id.
-    
-    assert (Z.pos modulus <> 0) by (pose proof Pos2Z.is_pos modulus; omega).
-    pose proof div_mod.
-    break_match; subst.
-    
-    rewrite Z.mul_0_r, Z.add_0_r, Z.sub_0_r.
-    (* TODO : how to prove second carry is 0? *)
-    rewrite Z.add_mod, B.Associational.eval_reduce by assumption.
-    autorewrite with uncps push_id push_basesystem_eval.
-    rewrite Hm. autorewrite with zsimplify.
-    reflexivity.
+    cbv [freeze_cps freeze mod_eq conditional_add_cps].
+    repeat progress autounfold.
+    autorewrite with uncps push_id.
 
+    match goal with |- context [B.Associational.reduce ?s ?c ?p] =>
+                    remember (B.Associational.reduce s c p) as y end.
+    match goal with |- context [fst ?x] =>
+                    remember x as carry_q end.
+    match goal with |- context [conditional_mask ?mask ?cond ?p] =>
+                    remember (conditional_mask mask cond p) as m0 end.
+    match goal with |- context [Columns.compact ?w ?p] =>
+                    remember (Columns.compact w p) as carry_r end.
+    destruct carry_q as [c0 z].
+    destruct carry_r as [c1 a].
     
-    ring_simplify.
-    let p := fresh "P" in
-    let carry := fresh "carry" in
-    let result := fresh "result" in
-    match goal with H:fst ?x <> 0 |- _ =>
-                         remember x as p; destruct p as [carry result];
-                           autorewrite with cancel_pair in *
-    end.
-    rewrite Columns.eval_from_associational by assumption.
-    autorewrite with uncps push_id push_basesystem_eval.
-    rewrite Hm.
-    Check Z.add_mod_full.
-    match goal with |- context [(?a + ?b - ?c + ?d) mod ?m] =>
-                    replace (a + b - c + d) with (b + (a-c) + d) by ring;
-                    rewrite (Z.add_mod_full _ d), (Z.add_mod_full _ (a-c))
-    end.
-    rewrite !Z.mod_same by assumption.
-    rewrite !Z.add_0_r, !Z.add_0_l.
-    rewrite !Z.mod_mod by assumption.
-    rewrite Z.sub_mod_full.
-    rewrite B.Associational.eval_reduce by assumption.
-    autorewrite with uncps push_id push_basesystem_eval.
+  Admitted.
+End Freeze.
     
 
   
